# Math 150:08
Date: 2017-09-26 09:10 - 11:00

## Derivatives

### Formulas
 1. $$f'(a)=\lim_{x \to a} \frac{f(x)-f(a)}{x-a}$$
 2. $$f'(a)=\lim_{h \to 0} \frac{f(a+h) - f(a)}{h}$$
 2. $$f'(x)=\lim_{h \to 0} \frac{f(x+h) - f(x)}{h}$$

### Ex. 1:
Given $f(x)=x^3$. Find $f'(2)$:
 - $$f'(2)=\lim_{x \to 2} \frac{f(x) - f(2)}{x - 2} = \lim_{x \to 2} \frac{x^3-2^3}{x-2} = \lim_{x \to 2}\frac{(x-2)(x^2+2x+4)}{(x-2)} = \lim_{x \to 2}(x^2+2x+4) = 2^2+2*2+4=12$$

### Ex. 2:
Given $f(x)=\sqrt{x+5}$
Find $f'(y)$
Using formula 2.
 - $$f'(4)=\lim_{h \to 0}\frac{f(y+h) - f(4)}{h} = \lim_{h \to 0}\frac{\sqrt{4+h}-\sqrt{9}}{h} = \lim_{h \to 0}\frac{(\sqrt{4+h} - \sqrt{9})(\sqrt{4+h} + \sqrt{9})}{(\sqrt{4+h} + \sqrt{9})}$$

### Ex. 3:
Given $f(x)=\frac{4}{x}+1$
Find $f'(3)$
 - $$f'(3)=\lim_{h \to 0}\frac{f(3+h)-f(3)}{h} = \lim_{h \to 0}\frac{(\frac{4}{3+h} + 1) - (\frac{4}{3}+1)}{h} = \lim_{h \to 0} \frac{(\frac{4}{3+h} - \frac{4}{3})}{h}$$
 - $$=\lim_{h\to 0}\frac{12 - (3+h)4}{(3+h)*3*h} = \lim_{h \to 0} \frac{-4h}{(3+h)*3} = \lim_{h \to 0} \frac{-4}{(3+h) * 3}=-\frac{4}{9}$$

## Derivative as a Function
$$f'(a) =\lim_{h \to 0} \frac{f(a+h) - f(a)}{h}$$
$$a \to f'(a)$$
$$x \to f'(x)$$
